\section{Electromagnetic Theory}

\subsection{Maxwell's Equations}
In a homogeneous region with permittivity $\varepsilon$ and permeability $\mu$, Maxwell's equations describe the electric fields $\vec{E}, \vec{D}$ and magnetic fields $\vec{H}, \vec{B}$.
\begin{align}
	\nabla \times \vec{E} & = -j\omega\mu\vec{H}, \label{eq:maxwell_E} \\
	\nabla \times \vec{H} & = j\omega\varepsilon\vec{E} + \vec{J}_0, \label{eq:maxwell_H} \\
	\nabla \cdot \vec{D} & = \rho, \label{eq:maxwell_D} \\
	\nabla \cdot \vec{B} & = 0, \label{eq:maxwell_B}
\end{align}
where $\vec{B} = \mu \vec{H}$ and $\vec{D} = \varepsilon \vec{E}$. Throughout the text, we assume a time-harmonic formulation with time dependence $e^{j\omega t}$.

\subsection{Green's Functions}
A Green's function is the impulse response of a linear differential equations on a specified domain. Using the superposition principle, the solution of a differential equation can be expressed as a sum of Green's functions. This property will allow us to write an integral equation for the electric field in Section~\ref{sec:em_efie}.

\subsubsection{Electrostatic Green's Function}
Consider the electrostatic Poisson equation
\begin{equation}
	\nabla^2 \phi = -\frac{\rho}{\varepsilon},
\end{equation}
where $\rho$ is the charge density. We can apply the Green's function method as outlined above to find the electric potential due to an arbitrary charge configuration. First, we find the impulse response $G(r)$ such that
\begin{equation}
	\nabla^2 G(\vecr) = -\frac{\delta(\vecr)}{\varepsilon}.
\end{equation}
Expanding the Laplace operator in spherical coordinates, we find
\begin{equation*}
	\nabla^2 G = \frac{1}{r^2} \frac{\partial}{\partial r} \left[ r^2 \frac
	{\partial G}{\partial r} \right] = \frac{\partial^2 G}{\partial r^2} + \frac{2}{r} \frac{\partial G}{\partial r} = \frac{1}{r} \frac{\partial^2 (r G)}{\partial r^2}
\end{equation*}
Outside of the point $r = 0$, the Dirac delta function is zero, such that
\begin{equation}
	\frac{\partial^2 (r G)}{\partial r^2} = 0 \qquad r > 0
\end{equation}
Integrating this differential equation twice gives us the general solution $G(r) = a + \frac{b}{r}$. We must have $G \to 0$ as $r \to \infty$, so the coefficient $a = 0$. To find coefficient $b$, we integrate the differential equation over a sphere of radius $R$:
\begin{align*}
	b \iiint_{V} \nabla^2 \left( \frac{1}{r} \right) dV & = - \iiint_V \frac{\delta(r)}{\varepsilon} dV = -\frac{1}{\varepsilon} \\
	\oiint_{\partial V} \nabla \left( \frac{1}{r} \right) \cdot \hat{\vecr} ds & = -\frac{1}{\varepsilon b} \\
	\oiint_{\partial V} \frac{1}{r^2} ds & = \frac{1}{\varepsilon b} \\
	4\pi & = \frac{1}{\varepsilon b}
\end{align*}
Therefore, the electrostatic Green's function becomes
\begin{equation}
	G(\vecr, \vecrp) = \frac{1}{4\pi \varepsilon r}, \qquad r = |\vecr - \vecrp|.
\end{equation}
Then, the electric potential due to an arbitrary charge distribution $\rho(\vecr)$ is 
\begin{equation}
	\phi(\vecr) = \iiint G(\vecr, \vecrp) \rho(\vecrp) d\vecrp = \frac{1}{4\pi\varepsilon} \iiint \frac{\rho(\vecrp)}{|\vecr - \vecrp|} d\vecrp
\end{equation}

\subsubsection{Electrodynamic Green's Function}
Similarly, we can derive a Green's function which satisfies the scalar Helmholtz equation. It will be shown later that the electrodynamic equations resemble the (vector) Helmholtz equation. Consider
\begin{equation}
	\nabla^2 G(\vecr, \vecrp) + k^2 G(\vecr, \vecrp) = -\delta(\vecr, \vecrp)
\end{equation}
Using the same derivation as before, we can equate the left-hand side to zero for $r > 0$.
\begin{equation}
	\frac{\partial^2 (r G)}{\partial r^2} + k^2 (r G) = 0 \qquad r > 0
\end{equation}
The solution to this differential equation is
\begin{equation*}
	G(r) = \frac{a e^{-j k r}}{r} + \frac{b e^{+j k r}}{r}.
\end{equation*}
By requiring that $G \to 0$ as $r \to \infty$, we find that $b = 0$. To find coefficient $a$, we again integrate over a sphere of radius $R$.
\begin{equation*}
	a \iiint_V \nabla^2 \left( \frac{e^{-jkr}}{r} \right) + k^2 \left( \frac{e^{-jkr}}{r} \right) dV = -1
\end{equation*}
The first part of the integral can be tackled by applying the divergence theorem:
\begin{align*}
	\iiint_V \nabla^2 \left( \frac{e^{-jkr}}{r} \right) dV & = \oiint_{\partial V} \nabla \left( \frac{e^{-jkr}}{r} \right) \cdot \hat{\vecr} ds = 4\pi a^2 \left[ \frac{\partial}{\partial r} \left( \frac{e^{-jkr}}{r} \right) \right]_{r = R} \\
	\lim_{R \to 0} 4\pi a^2 \left[ \frac{\partial}{\partial r} \left( \frac{e^{-jkr}}{r} \right) \right]_{r = R} & = -4\pi
\end{align*}
The second part of the integral is calculated by inspection:
\begin{align*}
	\iiint_V k^2 \left( \frac{e^{-jkr}}{r} \right) dV & = 4\pi k^2 R^2 \int_0^R \frac{e^{-jkr}}{r} dr \\
	\lim_{R \to 0} 4\pi k^2 R^2 \int_0^R \frac{e^{-jkr}}{r} dr & = 0
\end{align*}
Therefore, we find that the coefficient $a = \frac{1}{4\pi}$ and the electrodynamic Green's function is
\begin{equation}
	G(\vecr, \vecrp) = \frac{e^{-jkr}}{4\pi r}, \qquad r = |\vecr - \vecrp|.
\end{equation}

\subsection{Electric Field Integral Equation (EFIE)}
\label{sec:em_efie}
Taking the curl of (\ref{eq:maxwell_E}) we obtain
\begin{equation*}
	\nabla \times \nabla \times \vec{E}  = -j\omega\mu (j\omega\varepsilon \vec{E} + \vec{J}) = \nabla (\nabla \cdot \vec{E}) - \nabla^2 \vec{E}
\end{equation*}
Gathering the unknown $\vec{E}$ on the left-hand side, and the source terms involving $\vec{J}$ on the right:
\begin{equation}
	\nabla^2 \vec{E} + k^2 \vec{E} = j\omega\mu\vec{J} - \frac{\nabla (\nabla \cdot \vec{J})}{j\omega\varepsilon}
\end{equation}
This equation has the vector Helmholtz form with wavenumber $k = \nicefrac{\omega}{c} = \omega \sqrt{\mu \varepsilon}$. Using the electrodynamic Green's function derived above, we get an integral equation for the electric field.
\begin{equation}
	\vec{E}(\vecr) = -j\omega\mu \iiint G(\vecr, \vecrp) \left[ 1 + \frac
	{\nabla^\prime \nabla^\prime}{k^2} \right] \vec{J}(\vecrp) d\vecrp
	\label{eq:efie}
\end{equation}
Equation (\ref{eq:efie}) is called the \emph{electric field integral equation} (EFIE) and can also be written more compactly in terms of the operator $\oL$.
\begin{equation}
	\vec{E}(\vecr) = -j\omega\mu (\oL \vec{J})(\vecr),
\end{equation}
where
\begin{equation}
	(\oL\vec{X})(\vecr) = \iiint G(\vecr, \vecrp) \left[ 1 + \frac{\nabla^\prime \nabla^\prime}{k^2} \right] \vec{X}(\vecrp) d\vecrp
\end{equation}
Let the total electric field be written as a combination of the scattered field (due to an induced current density $\vec{J}$) and the incident field: $\vec{E} = \vec{E}^{s} + \vec{E}^{i}$. At the boundary of a conducting surface $S$, the following holds:
\begin{equation}
	\hat{\vec{n}}(\vecr) \times \left[ \vec{E}^i(\vecr) + \vec{E}^s(\vecr) \right] = 0,
\end{equation}
where $\hat{\vec{n}}(\vecr)$ is the surface normal at $\vecr \in S$. Thus, we can rewrite the ``surface'' integral equation as
\begin{equation}
	-\hat{\vec{n}}(\vecr) \times \vec{E}^i(\vecr) = \hat{\vec{n}}(\vecr) \times -j\omega\mu(\oL \vec{J})(\vecr)
\end{equation}
Finally, we can drop the $\hat{\vec{n}} \times$ and implicitly assume that the vectorial quantities are tangential to the conducting surface.
\begin{equation}
	\vec{E}^i(\vecr) = j\omega\mu(\oL \vec{J})(\vecr)
	\label{eq:surf_efie}
\end{equation}
Observe that this equation is very similar to the original EFIE in (\ref{eq:efie}), but with a reversed sign. The domain of integration is now restricted to the conducting surfaces.